match val threaded through everything but OeufProof

src/FlatCompCombined.v
@@ -18,23 +18,427 @@ Require
     FlatIntTagComp
 .
 
+Definition compile_seq (cu : LocalsOnly.prog_type) : res FlatSeq.prog_type :=
+  OK cu
+  @@ FlatSwitchComp.compile_cu
+  @@ FlatSeqComp.compile_cu.
+
+Section FSIMseq.
+
+  Variable a : LocalsOnly.prog_type.
+  Variable b : FlatSeq.prog_type.
+  Hypothesis TRANSF : compile_seq a = OK b.
+
+  Lemma compile_seq_succ :
+    { c | FlatSwitchComp.compile_cu a = c }.
+  Proof.
+    unfold compile_seq in TRANSF. break_result_chain. eauto.
+  Qed.
+  
+  Definition fsim_seq : Semantics.forward_simulation (LocalsOnly.semantics a) (FlatSeq.semantics b).
+    destruct compile_seq_succ.
+    eapply Semantics.compose_forward_simulation;
+      try eapply FlatSwitchComp.fsim; eauto;
+      try eapply FlatSeqComp.fsim; eauto.
+    unfold compile_seq in *; break_result_chain.
+    congruence.
+  Defined.
+
+  Lemma fsim_seq_match_val :
+    forall x y,
+      Semantics.fsim_match_val _ _ fsim_seq x y <-> eq x y.
+  Proof.
+    intros. unfold fsim_seq.
+    destruct compile_seq_succ.
+    erewrite Semantics.fsim_match_val_compose. repeat instantiate (1 := eq).
+    split; intros; repeat break_exists; repeat eexists; repeat break_and; eauto; try congruence.
+    erewrite FlatSwitchComp.match_val_eq.
+    intros; split; intros; congruence.
+    erewrite FlatSeqComp.match_val_eq.
+    intros; split; intros; congruence.
+  Qed.    
+
+End FSIMseq.
+
+Definition compile_seq2 (cu : LocalsOnly.prog_type) : res FlatSeq2.prog_type :=
+  OK cu
+  @@@ compile_seq
+  @@ FlatSeqComp2.compile_cu.
+
+Section FSIMseq2.
+
+  Variable a : LocalsOnly.prog_type.
+  Variable b : FlatSeq2.prog_type.
+  Hypothesis TRANSF : compile_seq2 a = OK b.
+
+  Lemma compile_seq2_succ :
+    { c | compile_seq a = Some c }.
+  Proof.
+    unfold compile_seq2 in TRANSF. break_result_chain. eauto.
+  Qed.
+  
+  Definition fsim_seq2 : Semantics.forward_simulation (LocalsOnly.semantics a) (FlatSeq2.semantics b).
+    destruct compile_seq2_succ.
+    eapply Semantics.compose_forward_simulation;
+      try eapply fsim_seq; eauto;
+      try eapply FlatSeqComp2.fsim; eauto.
+    unfold compile_seq2 in *; break_result_chain.
+    unfold option_to_res in *. congruence.
+  Defined.
+
+  Lemma fsim_seq2_match_val :
+    forall x y,
+      Semantics.fsim_match_val _ _ fsim_seq2 x y <-> eq x y.
+  Proof.
+    intros. unfold fsim_seq2.
+    destruct compile_seq2_succ.
+    erewrite Semantics.fsim_match_val_compose. repeat instantiate (1 := eq).
+    split; intros; repeat break_exists; repeat eexists; repeat break_and; eauto; try congruence.
+    intros. erewrite fsim_seq_match_val.
+    intros; split; intros; congruence.
+    erewrite FlatSeqComp2.match_val_eq.
+    intros; split; intros; congruence.
+  Qed.    
+
+End FSIMseq2.
+
+Definition compile_seqstmt (cu : LocalsOnly.prog_type) : res FlatSeqStmt.prog_type :=
+  OK cu
+  @@@ compile_seq2
+  @@ FlatSeqStmtComp.compile_cu.
+
+Section FSIMseqstmt.
+
+  Variable a : LocalsOnly.prog_type.
+  Variable b : FlatSeqStmt.prog_type.
+  Hypothesis TRANSF : compile_seqstmt a = OK b.
+
+  Lemma compile_seqstmt_succ :
+    { c | compile_seq2 a = Some c }.
+  Proof.
+    unfold compile_seqstmt in TRANSF. break_result_chain. eauto.
+  Qed.
+  
+  Definition fsim_seqstmt : Semantics.forward_simulation (LocalsOnly.semantics a) (FlatSeqStmt.semantics b).
+    destruct compile_seqstmt_succ.
+    eapply Semantics.compose_forward_simulation;
+      try eapply fsim_seq2; eauto;
+      try eapply FlatSeqStmtComp.fsim; eauto.
+    unfold compile_seqstmt in *; break_result_chain.
+    unfold option_to_res in *. congruence.
+  Defined.
+
+  Lemma fsim_seqstmt_match_val :
+    forall x y,
+      Semantics.fsim_match_val _ _ fsim_seqstmt x y <-> eq x y.
+  Proof.
+    intros. unfold fsim_seqstmt.
+    destruct compile_seqstmt_succ.
+    erewrite Semantics.fsim_match_val_compose. repeat instantiate (1 := eq).
+    split; intros; repeat break_exists; repeat eexists; repeat break_and; eauto; try congruence.
+    intros. erewrite fsim_seq2_match_val.
+    intros; split; intros; congruence.
+    erewrite FlatSeqStmtComp.match_val_eq.
+    intros; split; intros; congruence.
+  Qed.    
+
+End FSIMseqstmt.
+
+Definition compile_return (cu : LocalsOnly.prog_type) : res FlatReturn.prog_type :=
+  OK cu
+  @@@ compile_seqstmt
+  @@ FlatReturnComp.compile_cu.
+
+Section FSIMreturn.
+
+  Variable a : LocalsOnly.prog_type.
+  Variable b : FlatReturn.prog_type.
+  Hypothesis TRANSF : compile_return a = OK b.
+
+  Lemma compile_return_succ :
+    { c | compile_seqstmt a = Some c }.
+  Proof.
+    unfold compile_return in TRANSF. break_result_chain. eauto.
+  Qed.
+  
+  Definition fsim_return : Semantics.forward_simulation (LocalsOnly.semantics a) (FlatReturn.semantics b).
+    destruct compile_return_succ.
+    eapply Semantics.compose_forward_simulation;
+      try eapply fsim_seqstmt; eauto;
+      try eapply FlatReturnComp.fsim; eauto.
+    unfold compile_return in *; break_result_chain.
+    unfold option_to_res in *. congruence.
+  Defined.
+
+  Lemma fsim_return_match_val :
+    forall x y,
+      Semantics.fsim_match_val _ _ fsim_return x y <-> eq x y.
+  Proof.
+    intros. unfold fsim_return.
+    destruct compile_return_succ.
+    erewrite Semantics.fsim_match_val_compose. repeat instantiate (1 := eq).
+    split; intros; repeat break_exists; repeat eexists; repeat break_and; eauto; try congruence.
+    intros. erewrite fsim_seqstmt_match_val.
+    intros; split; intros; congruence.
+    erewrite FlatReturnComp.match_val_eq.
+    intros; split; intros; congruence.
+  Qed.    
+
+End FSIMreturn.
+
+Definition compile_expr (cu : LocalsOnly.prog_type) : res FlatExpr.prog_type :=
+  OK cu
+  @@@ compile_return
+  @@ FlatExprComp.compile_cu.
+
+Section FSIMexpr.
+
+  Variable a : LocalsOnly.prog_type.
+  Variable b : FlatExpr.prog_type.
+  Hypothesis TRANSF : compile_expr a = OK b.
+
+  Lemma compile_expr_succ :
+    { c | compile_return a = Some c }.
+  Proof.
+    unfold compile_expr in TRANSF. break_result_chain. eauto.
+  Qed.
+  
+  Definition fsim_expr : Semantics.forward_simulation (LocalsOnly.semantics a) (FlatExpr.semantics b).
+    destruct compile_expr_succ.
+    eapply Semantics.compose_forward_simulation;
+      try eapply fsim_return; eauto;
+      try eapply FlatExprComp.fsim; eauto.
+    unfold compile_expr in *; break_result_chain.
+    unfold option_to_res in *. congruence.
+  Defined.
+
+  Lemma fsim_expr_match_val :
+    forall x y,
+      Semantics.fsim_match_val _ _ fsim_expr x y <-> eq x y.
+  Proof.
+    intros. unfold fsim_expr.
+    destruct compile_expr_succ.
+    erewrite Semantics.fsim_match_val_compose. repeat instantiate (1 := eq).
+    split; intros; repeat break_exists; repeat eexists; repeat break_and; eauto; try congruence.
+    intros. erewrite fsim_return_match_val.
+    intros; split; intros; congruence.
+    erewrite FlatExprComp.match_val_eq.
+    intros; split; intros; congruence.
+  Qed.    
+
+End FSIMexpr.
+
+Definition compile_exprret (cu : LocalsOnly.prog_type) : res FlatExprRet.prog_type :=
+  OK cu
+  @@@ compile_expr
+  @@ FlatExprRetComp.compile_cu.
+
+Section FSIMexprret.
+
+  Variable a : LocalsOnly.prog_type.
+  Variable b : FlatExprRet.prog_type.
+  Hypothesis TRANSF : compile_exprret a = OK b.
+
+  Lemma compile_exprret_succ :
+    { c | compile_expr a = Some c }.
+  Proof.
+    unfold compile_exprret in TRANSF. break_result_chain. eauto.
+  Qed.
+  
+  Definition fsim_exprret : Semantics.forward_simulation (LocalsOnly.semantics a) (FlatExprRet.semantics b).
+    destruct compile_exprret_succ.
+    eapply Semantics.compose_forward_simulation;
+      try eapply fsim_expr; eauto;
+      try eapply FlatExprRetComp.fsim; eauto.
+    unfold compile_exprret in *; break_result_chain.
+    unfold option_to_res in *. congruence.
+  Defined.
+
+  Lemma fsim_exprret_match_val :
+    forall x y,
+      Semantics.fsim_match_val _ _ fsim_exprret x y <-> eq x y.
+  Proof.
+    intros. unfold fsim_exprret.
+    destruct compile_exprret_succ.
+    erewrite Semantics.fsim_match_val_compose. repeat instantiate (1 := eq).
+    split; intros; repeat break_exists; repeat eexists; repeat break_and; eauto; try congruence.
+    intros. erewrite fsim_expr_match_val.
+    intros; split; intros; congruence.
+    erewrite FlatExprRetComp.match_val_eq.
+    intros; split; intros; congruence.
+  Qed.    
+
+End FSIMexprret.
+
+Definition compile_stop (cu : LocalsOnly.prog_type) : res FlatStop.prog_type :=
+  OK cu
+  @@@ compile_exprret
+  @@ FlatStopComp.compile_cu.
+
+Section FSIMstop.
+
+  Variable a : LocalsOnly.prog_type.
+  Variable b : FlatStop.prog_type.
+  Hypothesis TRANSF : compile_stop a = OK b.
+
+  Lemma compile_stop_succ :
+    { c | compile_exprret a = Some c }.
+  Proof.
+    unfold compile_stop in TRANSF. break_result_chain. eauto.
+  Qed.
+  
+  Definition fsim_stop : Semantics.forward_simulation (LocalsOnly.semantics a) (FlatStop.semantics b).
+    destruct compile_stop_succ.
+    eapply Semantics.compose_forward_simulation;
+      try eapply fsim_exprret; eauto;
+      try eapply FlatStopComp.fsim; eauto.
+    unfold compile_stop in *; break_result_chain.
+    unfold option_to_res in *. congruence.
+  Defined.
+
+  Lemma fsim_stop_match_val :
+    forall x y,
+      Semantics.fsim_match_val _ _ fsim_stop x y <-> eq x y.
+  Proof.
+    intros. unfold fsim_stop.
+    destruct compile_stop_succ.
+    erewrite Semantics.fsim_match_val_compose. repeat instantiate (1 := eq).
+    split; intros; repeat break_exists; repeat eexists; repeat break_and; eauto; try congruence.
+    intros. erewrite fsim_exprret_match_val.
+    intros; split; intros; congruence.
+    erewrite FlatStopComp.match_val_eq.
+    intros; split; intros; congruence.
+  Qed.    
+
+End FSIMstop.
+
+Definition compile_destcheck (cu : LocalsOnly.prog_type) : res FlatDestCheck.prog_type :=
+  OK cu
+  @@@ compile_stop
+  @@@ FlatDestCheckComp.compile_cu.
+
+Section FSIMdestcheck.
+
+  Variable a : LocalsOnly.prog_type.
+  Variable b : FlatDestCheck.prog_type.
+  Hypothesis TRANSF : compile_destcheck a = OK b.
+
+  Lemma compile_destcheck_succ :
+    { c | compile_stop a = Some c }.
+  Proof.
+    unfold compile_destcheck in TRANSF. break_result_chain. eauto.
+  Qed.
+  
+  Definition fsim_destcheck : Semantics.forward_simulation (LocalsOnly.semantics a) (FlatDestCheck.semantics b).
+    destruct compile_destcheck_succ.
+    eapply Semantics.compose_forward_simulation;
+      try eapply fsim_stop; eauto;
+      try eapply FlatDestCheckComp.fsim; eauto.
+    unfold compile_destcheck in *; break_result_chain.
+    unfold option_to_res in *. congruence.
+  Defined.
+
+  Lemma fsim_destcheck_match_val :
+    forall x y,
+      Semantics.fsim_match_val _ _ fsim_destcheck x y <-> eq x y.
+  Proof.
+    intros. unfold fsim_destcheck.
+    destruct compile_destcheck_succ.
+    erewrite Semantics.fsim_match_val_compose. repeat instantiate (1 := eq).
+    split; intros; repeat break_exists; repeat eexists; repeat break_and; eauto; try congruence.
+    intros. erewrite fsim_stop_match_val.
+    intros; split; intros; congruence.
+    erewrite FlatDestCheckComp.match_val_eq.
+    intros; split; intros; congruence.
+  Qed.    
+
+End FSIMdestcheck.
+
+
+Definition compile_inttag (cu : LocalsOnly.prog_type) : res FlatIntTag.prog_type :=
+  OK cu
+  @@@ compile_destcheck
+  @@@ FlatIntTagComp.compile_cu.
+
+Section FSIMinttag.
+
+  Variable a : LocalsOnly.prog_type.
+  Variable b : FlatIntTag.prog_type.
+  Hypothesis TRANSF : compile_inttag a = OK b.
+
+  Lemma compile_inttag_succ :
+    { c | compile_destcheck a = Some c }.
+  Proof.
+    unfold compile_inttag in TRANSF. break_result_chain. eauto.
+  Qed.
+  
+  Definition fsim_inttag : Semantics.forward_simulation (LocalsOnly.semantics a) (FlatIntTag.semantics b).
+    destruct compile_inttag_succ.
+    eapply Semantics.compose_forward_simulation;
+      try eapply fsim_destcheck; eauto;
+      try eapply FlatIntTagComp.fsim; eauto.
+    unfold compile_inttag in *; break_result_chain.
+    unfold option_to_res in *. congruence.
+  Defined.
+
+  Lemma fsim_inttag_match_val :
+    forall x y,
+      Semantics.fsim_match_val _ _ fsim_inttag x y <-> FlatIntTagComp.I_value x y.
+  Proof.
+    intros. unfold fsim_inttag.
+    destruct compile_inttag_succ.
+    erewrite Semantics.fsim_match_val_compose.
+    Focus 2.
+    intros. erewrite fsim_destcheck_match_val.
+    intros; split; intros; congruence.
+    instantiate (1 := MatchValues.mv_high).
+    split; intros; repeat break_exists; repeat break_and.
+    erewrite fsim_destcheck_match_val in H. congruence.
+    eexists; split.
+    erewrite fsim_destcheck_match_val. reflexivity. eauto.
+    erewrite FlatIntTagComp.match_val_I_value.
+    intros; split; intros; congruence.
+  Qed.    
+
+End FSIMinttag.
+
+
+
 Module A := LocalsOnly.
 Module B := FlatIntTag.
 
 
 Definition compile_cu (cu : A.env * list metadata) : res (B.env * list metadata) :=
-  OK cu
-  @@ FlatSwitchComp.compile_cu
-  @@ FlatSeqComp.compile_cu
-  @@ FlatSeqComp2.compile_cu
-  @@ FlatSeqStmtComp.compile_cu
-  @@ FlatReturnComp.compile_cu
-  @@ FlatExprComp.compile_cu
-  @@ FlatExprRetComp.compile_cu
-  @@ FlatStopComp.compile_cu
- @@@ FlatDestCheckComp.compile_cu ~~ "FlatDestCheckComp"
- @@@ FlatIntTagComp.compile_cu ~~ "FlatIntTag"
-.
+  compile_inttag cu.
+
+
+
+Section Preservation.
+
+  Variable prog : A.prog_type.
+  Variable tprog : B.prog_type.
+
+  Hypothesis TRANSF : compile_cu prog = OK tprog.
+
+  Definition fsim :
+    Semantics.forward_simulation (A.semantics prog) (B.semantics tprog).
+  Proof.
+    eapply fsim_inttag. apply TRANSF.
+  Defined.
+
+
+  Lemma match_val_I_value :
+    forall x y,
+      Semantics.fsim_match_val _ _ fsim x y <-> FlatIntTagComp.I_value x y.
+  Proof.
+    unfold fsim. eapply fsim_inttag_match_val.
+  Qed.
+  
+End Preservation.
+
+
+
+
 
 Inductive I : A.state -> B.state -> Prop :=
 | ICombined : forall s00 s01 s02 s03 s04 s05 s06 s07 s08 s09 s10,
@@ -88,6 +492,18 @@ Theorem compile_I_func : forall a ameta b bmeta,
     Forall2 I_func a b.
 intros0 Hcomp. unfold compile_cu in *.
 
+unfold compile_inttag in *.
+unfold compile_destcheck in *.
+unfold compile_stop in *.
+unfold compile_exprret in *.
+unfold compile_expr in *.
+unfold compile_return in *.
+unfold compile_seqstmt in *.
+unfold compile_seq2 in *.
+unfold compile_seq in *.
+
+
+
 remember (a, ameta) as aprog.
 break_result_chain.
 subst aprog.  repeat on (_ * _)%type, fun x => destruct x.
@@ -108,49 +524,4 @@ Qed.
 
 
 
-Require Semantics.
 
-Section Preservation.
-
-  Variable prog : A.prog_type.
-  Variable tprog : B.prog_type.
-
-  Hypothesis TRANSF : compile_cu prog = OK tprog.
-
-  Theorem fsim :
-    Semantics.forward_simulation (A.semantics prog) (B.semantics tprog).
-  Proof.
-    unfold compile_cu in TRANSF.
-    break_result_chain.
-
-    eapply Semantics.compose_forward_simulation.
-    eapply FlatSwitchComp.fsim; try eassumption.
-
-    eapply Semantics.compose_forward_simulation.
-    eapply FlatSeqComp.fsim; try eassumption.
-
-    eapply Semantics.compose_forward_simulation.
-    eapply FlatSeqComp2.fsim; try eassumption.
-
-    eapply Semantics.compose_forward_simulation.
-    eapply FlatSeqStmtComp.fsim; try eassumption.
-
-    eapply Semantics.compose_forward_simulation.
-    eapply FlatReturnComp.fsim; try eassumption.
-
-    eapply Semantics.compose_forward_simulation.
-    eapply FlatExprComp.fsim; try eassumption.
-
-    eapply Semantics.compose_forward_simulation.
-    eapply FlatExprRetComp.fsim; try eassumption.
-
-    eapply Semantics.compose_forward_simulation.
-    eapply FlatStopComp.fsim; try eassumption.
-
-    eapply Semantics.compose_forward_simulation.
-    eapply FlatDestCheckComp.fsim; try eassumption.
-
-    eapply FlatIntTagComp.fsim; try eassumption.
-  Qed.
-
-End Preservation.
